poly: no need to expose kernel types!

src/lib/poly/Kuiper.HReduce.fst
@@ -42,6 +42,34 @@ let smin (a b : sz): sz =
   let open FStar.SizeT in
   if a <^ b then a else b
 
+(* Ownership of array r between i and j. The first value of that slice
+is the reduction of all the values in the (original) slice v. *)
+unfold
+let gpu_pts_to_slice_sum_inner
+  (#et:Type0) {| scalar et |}
+  (#sz:nat)
+  (r : gpu_array et sz)
+  (i j :nat)
+  (v : seq et)
+  (s : seq et)
+: slprop
+= gpu_pts_to_slice r i j s
+  ** pure (i < j /\ j <= sz /\
+           len v = sz /\
+           len s = j - i /\
+           squash (is_reduction zero add (Seq.slice v i j) (s @! 0))) // SQUASH VERY IMPORTANT!!
+
+(* Not easy to mark this unfold as it has a lambda (in the exists) *)
+let gpu_pts_to_slice_sum
+  (#et:Type0) {| scalar et |}
+  (#sz:nat)
+  ([@@@mkey] r: gpu_array et sz)
+  ([@@@mkey] i : nat)
+  (j:nat)
+  (v: seq et)
+: slprop
+= if_ (i < j && j <= sz) (exists* s. gpu_pts_to_slice_sum_inner r i j v s)
+
 // Barrier
 
 let barrier_matrix
@@ -121,6 +149,41 @@ fn mk_barrier_pre
     bigstar_map #_ #_ #0 #nth #(fun (i:nat { 0 <= i /\ i < nth }) -> emp) (fold_barrier_matrix_false nth r vv it tid);
   }
 }
+
+
+unfold
+let kpre
+  (#et:Type0) {| scalar et |}
+  (nth: nat) (a : gpu_array et nth) (s : erased (seq et))
+  (#_: squash (len s == nth)) (tid:nat{tid < nth})
+  : slprop =
+    gpu_pts_to_slice a tid (tid+1) seq![Seq.index s tid]
+
+unfold
+let kpost
+  (#et:Type0) {| scalar et |}
+  (nth: nat) (a : gpu_array et nth) (s : erased (seq et))
+  (#_: squash (len s == nth)) (tid:nat{tid < nth})
+  : slprop =
+    if_ (tid = 0) (gpu_pts_to_slice_sum a 0 nth s)
+
+type k_reduce_ty (et:Type0) {| scalar et |} =
+  (nth : szp { nth <= 1024 }) ->
+  (a : gpu_array et nth) ->
+  (#s :  erased (seq et)) ->
+  (#_: squash (Seq.length s == SZ.v nth)) ->
+  (etid : tid_t { (gdim_x etid <: nat) == 1 /\ (bdim_x etid <: nat) == SZ.v nth }) ->
+  stt unit
+  (requires
+    gpu **
+    thread_id etid **
+    mbarrier_tok nth (barrier_matrix nth a s) 0 (tidx_x etid) **
+    kpre nth a s (thread_index etid))
+  (ensures fun _ ->
+    gpu **
+    thread_id etid **
+    (exists* it. mbarrier_tok nth (barrier_matrix nth a s) it (tidx_x etid)) **
+    kpost nth a s (thread_index etid))
 
 // KrmlPrivate is essentially a "noextract". F* usually adds it
 // automatically to any definition that does not appear in the fsti,
