src/lib/poly/Kuiper.Softmax.fsti
@@ -5,41 +5,14 @@ open Kuiper
 
 module Vec = Pulse.Lib.Vec
 
-unfold
-type k_pointwise_exp_ty
-  (et:Type0) {| floating et |} =
-  (#lena : erased nat) ->
-  (a : gpu_array et lena) ->
-  (etid : tid_t { gdim_x etid == reveal lena /\ bdim_x etid == 1 }) ->
-  stt unit
-  (requires
-    gpu **
-    thread_id etid **
-    gpu_pts_to_array1 a (thread_index etid))
-  (ensures fun _ ->
-    gpu **
-    thread_id etid **
-    gpu_pts_to_array1 a (thread_index etid))
+inline_for_extraction
+val k_pointwise_exp_ty (et:Type0) {| floating et |} : Type0
 
 inline_for_extraction noextract
 val k_pointwise_exp (#et : Type0) {| floating et |} : k_pointwise_exp_ty et
 
-unfold
-type k_pointwise_div_ty
-  (et:Type0) {| floating et |} =
-  (#lena : erased nat) ->
-  (a : gpu_array et lena) ->
-  (d : et) ->
-  (etid : tid_t { gdim_x etid == reveal lena /\ bdim_x etid == 1 }) ->
-  stt unit
-  (requires
-    gpu **
-    thread_id etid **
-    gpu_pts_to_array1 a (thread_index etid))
-  (ensures fun _ ->
-    gpu **
-    thread_id etid **
-    gpu_pts_to_array1 a (thread_index etid))
+inline_for_extraction
+val k_pointwise_div_ty (et:Type0) {| floating et |} : Type0
 
 inline_for_extraction noextract
 val k_pointwise_div (#et : Type0) {| floating et |} : k_pointwise_div_ty et
